examples/loops: Add array predicates and reflective map tactic

src/Rupicola/Lib/Loops.v
@@ -1,17 +1,18 @@
 Require Import Arith PeanoNat.
 Require Import Coq.Program.Wf.
-Require Import Psatz.
+Require Import Coq.micromega.Psatz.
+Require Coq.Vectors.Vector.
+Require Import Coq.Setoids.Setoid.
+Require Import AdmitAxiom.
 
 Require Import Rupicola.Lib.Api.
+Require Import Rupicola.Examples.Cells.Cells.
 
-Definition nlet {A P} (vars: list string) (val : A) (body : forall a : A, P a) : P val :=
-  let x := val in body x.
-
-(* Set Primitive Projections. *)
-Record p2 {A B} := P2 { pfst: A; psnd: B }.
-(* Unset Primitive Projections. *)
-Arguments P2 {A B} pfst psnd: assert.
-Arguments p2: clear implicits.
+(* (* Set Primitive Projections. *) *)
+(* Record p2 {A B} := P2 { pfst: A; psnd: B }. *)
+(* (* Unset Primitive Projections. *) *)
+(* Arguments P2 {A B} pfst psnd: assert. *)
+(* Arguments p2: clear implicits. *)
 
 Lemma extends_refl {p o} {map: map.map p o} m:
   map.extends m m.
@@ -21,46 +22,6 @@ Lemma extends_eq {p o} {map: map.map p o} m1 m2:
   m1 = m2 ->
   map.extends m1 m2.
 Proof. intros * ->; apply extends_refl. Qed.
-
-(* FIXME Error: Anomaly "Uncaught exception Failure("hd")." until 8.13 *)
-(* Notation "'let/n' x := val 'in' body" := *)
-(*   (nlet [_] val (fun x => body)) *)
-(*     (at level 200, x ident, body at level 200, *)
-(*      format "'let/n'  x  :=  val  'in' '//' body", *)
-(*      only printing). *)
-
-Notation "'let/n' x 'as' nm := val 'in' body" :=
-  (nlet (P := fun _ => _) (* Force non-dependent type *)
-        [nm] val (fun x => body))
-    (at level 200, x ident, body at level 200,
-     format "'let/n'  x  'as'  nm  :=  val  'in' '//' body").
-
-Notation "'let/n' x := val 'in' body" :=
-  (nlet (P := fun _ => _) (* Force non-dependent type *)
-        [IdentParsing.binder_to_string val x]
-        val (fun x => body))
-    (at level 200, x ident, body at level 200,
-     only parsing).
-
-(* Notation "'let/n' ( x , y ) := val 'in' body" := *)
-(*   (nlet [_; _] val (fun '(x, y) => body)) *)
-(*     (at level 200, x ident, body at level 200, *)
-(*      format "'let/n'  ( x ,  y )  :=  val  'in' '//' body", *)
-(*      only printing). *)
-
-Notation "'let/n' ( x , y ) 'as' ( nx , ny ) := val 'in' body" :=
-  (nlet (P := fun _ => _) (* Force non-dependent type *)
-        [nx; ny] val (fun '(P2 x y) => body))
-    (at level 200, x ident, body at level 200,
-     format "'let/n'  ( x ,  y )  'as'  ( nx ,  ny )  :=  val  'in' '//' body").
-
-Notation "'let/n' ( x , y ) := val 'in' body" :=
-  (nlet (P := fun _ => _) (* Force non-dependent type *)
-        [IdentParsing.binder_to_string (pfst val) x;
-         IdentParsing.binder_to_string (psnd val) y]
-        val (fun '(P2 x y) => body))
-    (at level 200, x ident, y ident, body at level 200,
-     only parsing).
 
 Module Type ExitToken_sig.
   Axiom t : Set.
@@ -76,8 +37,9 @@ Module ExitToken <: ExitToken_sig.
   Definition set (tok: t) : t := true.
 End ExitToken.
 
-Class HasDefault (T: Type) := t: T.
-Class Convertible (T1 T2: Type) := to_nat: T1 -> T2.
+Class HasDefault (T: Type) := default: T.
+
+Class Convertible (T1 T2: Type) := cast: T1 -> T2.
 
 Fixpoint replace_nth {A} (n: nat) (l: list A) (a: A) {struct l} :=
   match l, n with
@@ -86,73 +48,213 @@ Fixpoint replace_nth {A} (n: nat) (l: list A) (a: A) {struct l} :=
   | h :: t, S n => h :: replace_nth n t a
   end.
 
-Lemma replace_nth_length {A} n (l: list A) a:
-  List.length (replace_nth n l a) = List.length l.
+Lemma nth_replace_nth {A}:
+  forall (xs: list A) idx idx' d v,
+    idx' = idx ->
+    idx < List.length xs ->
+    nth idx' (replace_nth idx xs v) d = v.
 Proof.
-  revert n; induction l; cbn; intros.
-  - reflexivity.
-  - destruct n; simpl; rewrite ?IHl; reflexivity.
+  intros; subst; revert dependent idx; revert dependent xs.
+  induction xs; cbn; intros idx Hlt.
+  - inversion Hlt.
+  - destruct idx; simpl.
+    + reflexivity.
+    + apply IHxs; auto with arith.
 Qed.
 
-Module FlatArray.
-  Section FlatArray.
+Lemma replace_nth_length {A}:
+  forall (l: list A) n a,
+    List.length (replace_nth n l a) = List.length l.
+Proof.
+  induction l; cbn; intros.
+  - reflexivity.
+  - destruct n; simpl; rewrite ?IHl; try reflexivity.
+Qed.
+
+Lemma Vector_to_list_length {T n}:
+  forall (v: Vector.t T n),
+    List.length (Vector.to_list v) = n.
+Proof.
+  induction v; cbn.
+  - reflexivity.
+  - f_equal; assumption.
+Qed.
+
+Lemma Vector_nth_hd_skipn {T n}:
+  forall (f: Fin.t n) idx (v : Vector.t T n) (t0 : T),
+    idx = proj1_sig (Fin.to_nat f) ->
+    Vector.nth v f = List.hd t0 (List.skipn idx (Vector.to_list v)).
+Proof.
+  induction f; cbn; intros; rewrite (Vector.eta v).
+  - subst; reflexivity.
+  - subst; destruct (Fin.to_nat f); cbn.
+    erewrite IHf; reflexivity.
+Qed.
+
+Lemma Vector_to_list_app {A n1 n2} :
+  forall v1 v2,
+    Vector.to_list (@Vector.append A n1 n2 v1 v2) =
+    List.app (Vector.to_list v1) (Vector.to_list v2).
+Proof.
+  induction v1; cbn; intros.
+  - reflexivity.
+  - f_equal. apply IHv1.
+Qed.
+
+Open Scope list_scope.
+
+Lemma List_firstn_app_l {A} :
+  forall (l1 l2: list A) n,
+    n = List.length l1 ->
+    List.firstn n (l1 ++ l2) = l1.
+Proof.
+  intros; subst.
+  rewrite List.firstn_app, List.firstn_all, Nat.sub_diag; simpl.
+  rewrite app_nil_r; reflexivity.
+Qed.
+
+Lemma List_firstn_app_l2 {A} :
+  forall (l1 l2: list A) n k,
+    n = List.length l1 ->
+    (List.firstn (n + k) (l1 ++ l2) = l1 ++ (List.firstn k l2)).
+Proof.
+  intros; subst.
+  rewrite List.firstn_app, List.firstn_all2, minus_plus; simpl; (reflexivity || lia).
+Qed.
+
+Lemma List_skipn_app_r {A} :
+  forall (l1 l2: list A) n,
+    n = List.length l1 ->
+    List.skipn n (l1 ++ l2) = l2.
+Proof.
+  intros; subst.
+  rewrite List.skipn_app, List.skipn_all, Nat.sub_diag; simpl; reflexivity.
+Qed.
+
+Lemma List_skipn_app_r2 {A} :
+  forall (l1 l2: list A) n k,
+    n = List.length l1 ->
+    List.skipn (n + k) (l1 ++ l2) =
+    List.skipn k l2.
+Proof.
+  intros; subst.
+  rewrite List.skipn_app, List.skipn_all, minus_plus; simpl; (reflexivity || lia).
+Qed.
+
+Lemma Vector_to_list_replace {A n}:
+  forall (a: Vector.t A n) (idx: nat) (f: Fin.t n) v,
+    idx = proj1_sig (Fin.to_nat f) ->
+    Vector.to_list (Vector.replace a f v) =
+    replace_nth idx (Vector.to_list a) v.
+Proof.
+  intros; subst; induction f; cbn; intros; rewrite (Vector.eta a).
+  - reflexivity.
+  - destruct (Fin.to_nat f); cbn in *.
+    f_equal; apply IHf.
+Qed.
+
+Lemma replace_nth_eqn {A} :
+  forall (xs: list A) idx x,
+    idx < List.length xs ->
+    replace_nth idx xs x =
+    List.firstn idx xs ++ x :: List.skipn (S idx) xs.
+Proof.
+  induction xs; cbn; intros idx x Hlt.
+  - inversion Hlt.
+  - destruct idx.
+    + reflexivity.
+    + cbn [List.firstn List.app].
+      f_equal; apply IHxs.
+      auto with arith.
+Qed.
+
+Lemma Vector_nth_replace {T n}:
+  forall (idx: Fin.t n) (v: Vector.t T n) (val: T),
+    Vector.nth (Vector.replace v idx val) idx = val.
+Proof.
+  induction idx; intros; rewrite (Vector.eta v); cbn; try rewrite IHidx; reflexivity.
+Qed.
+
+Module VectorArray.
+  Section VectorArray.
     Context {K V: Type}.
-    Context {v0: HasDefault V}.
-    Context {k2n: Convertible K nat}.
+    Context {Conv: Convertible K nat}.
+
+    Definition t n := Vector.t V n.
+    Definition get {n} (a: t n) (k: K) (pr: cast k < n) : V :=
+      Vector.nth_order a pr.
+    Definition put {n} (a: t n) (k: K) (pr: cast k < n) (v: V) : t n :=
+      Vector.replace_order a pr v.
+    (* FIXME needs an accessor that generates a test and returns a default *)
+  End VectorArray.
+
+  Arguments t : clear implicits.
+End VectorArray.
+
+Module ListArray.
+  Section ListArray.
+    Context {K V: Type}.
+    Context {HD: HasDefault V}.
+    Context {Conv: Convertible K nat}.
 
     Definition t := list V.
-    Definition get (a: t) (k: K) : V := nth_default v0 a (k2n k).
-    Definition put (a: t) (k: K) (v: V) : t := replace_nth (k2n k) a v.
-    (* FIXME needs a compilation rule for get_default which generates a test *)
-  End FlatArray.
-End FlatArray.
+    Definition get (a: t) (k: K) : V :=
+      List.nth (cast k) a default.
+    Definition put (a: t) (k: K) (v: V) : t :=
+      replace_nth (cast k) a v.
+    (* FIXME needs an accessor that generates a test and returns a default *)
+
+    Lemma put_length (a: t) (k: K) (v: V) :
+      List.length (put a k v) = List.length a.
+    Proof. intros; apply replace_nth_length. Qed.
+  End ListArray.
+
+  Arguments t : clear implicits.
+End ListArray.
 
 Section Gallina.
-  (* FIXME it's an interesting challenge here to decide what API “continue” should have. *)
-  Program Fixpoint ranged_for {A}
+  Context {A}
           (from to step: nat)
-          (body: forall (tok: ExitToken.t) (idx: nat) (acc: A), (ExitToken.t * A))
-          (a0: A) {measure (to - from)} : A :=
-    if le_gt_dec to from then a0
-    else let (tok, a0) := body (ExitToken.new true) from a0 in
+          (body: forall (tok: ExitToken.t) (idx: nat) (acc: A),
+              from <= idx < to -> (ExitToken.t * A))
+          (a0: A).
+
+  (* FIXME it's an interesting challenge here to decide what API “continue” should have. *)
+  Program Fixpoint ranged_for' idx (_: from <= idx) {measure (to - idx)} : A :=
+    if le_gt_dec to idx then a0
+    else let (tok, a0) := body (ExitToken.new true) idx a0 _ in
          if ExitToken.get tok then
-           ranged_for (from + S (pred step)) to step body a0
+           ranged_for' (idx + S (pred step)) _
          else a0.
-  Next Obligation.
-    lia.
-  Defined.
+  Next Obligation. lia. Qed.
+  Next Obligation. lia. Qed.
+
+  Definition ranged_for :=
+    ranged_for' from ltac:(auto).
 End Gallina.
 
 Section Compile.
   Context {semantics : Semantics.parameters}
           {semantics_ok : Semantics.parameters_ok semantics}.
 
-  Definition ranged_for_w {A}
-             (from to step: word)
-             (body: forall (tok: ExitToken.t) (idx: word) (acc: A), (ExitToken.t * A))
-             (a0: A) : A :=
+  Open Scope Z_scope.
+
+  Program Definition ranged_for_w {A}
+          (from to step: word)
+          (body: forall (tok: ExitToken.t) (idx: word) (acc: A),
+              word.unsigned from <= word.unsigned idx < word.unsigned to ->
+              (ExitToken.t * A))
+          (a0: A): A :=
     ranged_for (Z.to_nat (word.unsigned from))
                (Z.to_nat (word.unsigned to))
                (Z.to_nat (word.unsigned step))
-               (fun tok idx v =>
-                  body tok (word.of_Z (Z.of_nat idx)) v)
+               (fun tok idx acc pr =>
+                  body tok (word.of_Z (Z.of_nat idx)) acc _)
                a0.
-
-  (* Set Primitive Projections. *)
-  (* Record wp_args := *)
-  (*   { Trace: Semantics.trace; *)
-  (*     Memory: Semantics.mem; *)
-  (*     Locals: Semantics.locals; *)
-  (*     Functions: list (String.string * (list String.string * list String.string * cmd.cmd)) }. *)
-
-  (* Definition wp_cmd body spec args := *)
-  (*   (WeakestPrecondition.cmd *)
-  (*      (WeakestPrecondition.call args.(Functions)) *)
-  (*      body *)
-  (*      (args.(Trace)) *)
-  (*      (args.(Memory)) *)
-  (*      (args.(Locals)) *)
-  (*      spec). *)
+  Next Obligation.
+    pose proof word.unsigned_range to.
+    rewrite word.unsigned_of_Z, word.wrap_small; lia.
+  Qed.
 
   Notation "<{ 'Trace' := tr ; 'Memory' := mem ; 'Locals' := locals ; 'Functions' := functions }> cmd <{ post }>" :=
     (WeakestPrecondition.cmd
@@ -166,38 +268,10 @@ Section Compile.
                '//' cmd
                '//' <{  '[hv' post ']'  }> ']'").
 
-  (* Programmer (or tactic script) should put bounds in locals before looping *)
+  (* FIXME Programmer (or tactic script) should put bounds in locals before looping *)
 
   Definition predicate :=
     Semantics.trace -> Semantics.mem -> Semantics.locals -> Prop.
-
-  Require Import Cells.Cells.
-
-  Definition incr_gallina_spec (c: cell) : cell :=
-      let/n one := word.of_Z 1 in
-      let/n from := word.of_Z 3 in
-      let/n to := word.of_Z 5 in
-      let/n step := word.of_Z 1 in
-      let/n tick := word.of_Z 0 in
-      let/n (tick, c) :=
-         ranged_for_w (A := p2 word cell)
-                      from to step
-                      (fun tok idx '(P2 tick c) =>
-                         let/n v := get c in
-                         let/n v := word.add v idx in
-                         let/n c := put v c in
-                         let/n tick := word.add tick one in
-                         let/n from := to in
-                         (tok, (P2 tick c)))
-                      (P2 tick c) : p2 word cell in
-      (let/n v := get c in
-       let/n v := word.add v tick in
-       let/n c := put v c in
-       c).
-
-  Print incr_gallina_spec.
-
-  Local Infix "~>" := cell_value.
 
   (* FIXME find the way to preserve the name of the binder in ‘k’ instead of renaming everything to ‘head’ *)
 
@@ -335,29 +409,56 @@ Section Compile.
       eassumption. }
   Qed.
 
-  Arguments FlatArray.t V : clear implicits.
+  Section WordArray.
+    Context
+      {A K} (to_list: A -> list word) (to_word: K -> word)
+      (get: A -> K -> word)
+      (put: A -> K -> word -> A)
+      (repr: address -> A -> Semantics.mem -> Prop).
 
-  Definition word_array_value (addr: address) (a: FlatArray.t word) : Semantics.mem -> Prop :=
-    array scalar (word.of_Z (Memory.bytes_per_word Semantics.width)) addr a.
+    Notation to_nat idx := (Z.to_nat (word.unsigned (to_word idx))).
 
-  Instance Convertible_word_Nat : Convertible word nat :=
-    fun w => Z.to_nat (word.unsigned w).
-  Instance HasDefault_word : HasDefault word :=
-    word.of_Z 0.
+    Context (locals : Semantics.locals) (mem : Semantics.mem) (tr : Semantics.trace)
+            (R : Semantics.mem -> Prop)
+            (functions : list (string * (list string * list string * cmd)))
+            (T : Type) (pred : T -> predicate)
+            (a : A) (a_ptr : word) (a_var : string)
+            (val: word) (val_var: string)
+            (idx : K) (idx_var : string).
 
-  Lemma compile_wordarray_get :
-    forall (locals: Semantics.locals) (mem: Semantics.mem)
-      tr R functions
-      T (pred: T -> predicate)
-      a a_ptr a_var idx idx_var k k_impl var,
+    Context
+      (Hget: forall a,
+         exists default,
+           get a idx =
+           List.hd default (List.skipn (to_nat idx) (to_list a)))
+      (Hput:
+         (to_nat idx < List.length (to_list a))%nat ->
+         to_list (put a idx val) =
+         List.app
+           (List.firstn (to_nat idx) (to_list a))
+           (val :: List.skipn (S (to_nat idx)) (to_list a)))
+      (Hgetput:
+         (to_nat idx < List.length (to_list a))%nat ->
+         get (put a idx val) idx = val)
+      (Hrw:
+         Lift1Prop.iff1
+           (repr a_ptr a)
+           (array scalar (word.of_Z (Memory.bytes_per_word Semantics.width))
+                  a_ptr (to_list a)))
+      (Hrw_put:
+         Lift1Prop.iff1
+           (repr a_ptr (put a idx val))
+           (array scalar (word.of_Z (Memory.bytes_per_word Semantics.width))
+                  a_ptr (to_list (put a idx val)))).
 
-      sep (word_array_value a_ptr a) R mem ->
+    Lemma compile_word_array_get (k : word -> T) (k_impl : cmd) (var : string):
+      (Z.to_nat (word.unsigned (to_word idx)) < Datatypes.length (to_list a))%nat ->
+
+      sep (repr a_ptr a) R mem ->
       map.get locals a_var = Some a_ptr ->
-      map.get locals idx_var = Some idx ->
+      map.get locals idx_var = Some (to_word idx) ->
 
-      (word.unsigned idx < Z.of_nat (List.length a))%Z ->
-
-      let v := (FlatArray.get a idx) in
+      let v := get a idx in
       (let v := v in
        <{ Trace := tr;
           Memory := mem;
@@ -381,42 +482,39 @@ Section Compile.
                                 (expr.var idx_var)))))
         k_impl
       <{ pred (nlet [var] v k) }>.
-  Proof.
-    unfold word_array_value; cbn; intros.
-    pose proof word.unsigned_range idx.
-    exists (FlatArray.get a idx); split; cbn; [ | assumption ].
-    exists a_ptr; split; [ eassumption | ]; cbn.
-    exists idx; split; [ eassumption | ]; cbn.
-    eexists; split; [ | reflexivity ].
+    Proof.
+      cbn; intros.
+      pose proof word.unsigned_range (to_word idx).
+      destruct (Hget a) as [default Hget0].
+      exists (get a idx); split; cbn; [ | assumption ].
+      exists a_ptr; split; [ eassumption | ]; cbn.
+      exists (to_word idx); split; [ eassumption | ]; cbn.
+      eexists; split; [ | reflexivity ].
 
-    eapply load_word_of_sep.
-    seprewrite_in open_constr:(array_index_nat_inbounds
-                                 _ _ _ _ (Z.to_nat (word.unsigned idx))) H;
-      [ lia | ].
+      eapply load_word_of_sep.
+      seprewrite_in Hrw H0.        (* FIXME seprewrite shouldn't rename *)
+      (* FIXME: BEDROCK2: Adding an extra "_" at the end shelves an inequality *)
+      once (seprewrite_in open_constr:(array_index_nat_inbounds
+                                         _ _ _ _ (Z.to_nat (word.unsigned (to_word idx)))) H6);
+        [ assumption | ].
 
-    repeat rewrite ?word.ring_morph_mul, ?word.of_Z_unsigned, ?Z2Nat.id in H6 by lia.
-    unfold FlatArray.get, Convertible_word_Nat, HasDefault_word, HasDefault.
-    rewrite List.hd_skipn_nth_default.
-    ecancel_assumption.
-  Qed.
+      repeat rewrite ?word.ring_morph_mul, ?Z2Nat.id, ?word.of_Z_unsigned, ?Z2Nat.id in H5 by lia.
+      rewrite Hget0.
+      ecancel_assumption.
+    Qed.
 
-  Lemma compile_wordarray_put :
-    forall (locals: Semantics.locals) (mem: Semantics.mem)
-      tr R functions
-      T (pred: T -> predicate)
-      a a_ptr a_var idx idx_var val val_var k k_impl var,
+    Lemma compile_word_array_put (k: A -> T) (k_impl: cmd) (var: string) :
+      (Z.to_nat (word.unsigned (to_word idx)) < Datatypes.length (to_list a))%nat ->
 
-      sep (word_array_value a_ptr a) R mem ->
+      sep (repr a_ptr a) R mem ->
       map.get locals a_var = Some a_ptr ->
-      map.get locals idx_var = Some idx ->
+      map.get locals idx_var = Some (to_word idx) ->
       map.get locals val_var = Some val ->
 
-      (word.unsigned idx < Z.of_nat (List.length a))%Z ->
-
-      let a := (FlatArray.put a idx val) in
+      let a := (put a idx val) in
       (let a := a in
        forall mem',
-         sep (word_array_value a_ptr a) R mem' ->
+         sep (repr a_ptr a) R mem' ->
          <{ Trace := tr;
             Memory := mem';
             Locals := locals;
@@ -438,47 +536,493 @@ Section Compile.
            (expr.var val_var))
         k_impl
       <{ pred (nlet [var] a k) }>.
-  Proof.
-    unfold word_array_value; cbn; intros.
-    pose proof word.unsigned_range idx.
-    eexists; split; cbn.
+    Proof.
+      cbn; intros.
+      pose proof word.unsigned_range (to_word idx).
+      destruct (Hget (put a idx val)) as [default Hget0].
+      eexists; split; cbn.
 
-    {
-    eexists; split; [ eassumption | ]; cbn.
-    eexists; split; [ eassumption | reflexivity ].
-    }
+      { eexists; split; [ eassumption | ]; cbn.
+        eexists; split; [ eassumption | reflexivity ]. }
 
-    { eexists; split; cbn.
-      { eexists; split; [ eassumption | reflexivity ]. }
-      { red.
-        seprewrite_in           (* FIXME: BEDROCK2: Adding an extra "_" at the end shelves an inequality *)
-          open_constr:(array_index_nat_inbounds
-                         _ _ _ _ (Z.to_nat (word.unsigned idx))) H;
-          [ lia | ].
-        instantiate (1 := HasDefault_word) in H7.
-        eapply store_word_of_sep.
-        { repeat rewrite ?word.ring_morph_mul, ?word.of_Z_unsigned, ?Z2Nat.id in H7 by lia.
-          ecancel_assumption. }
-        { intros m Hm.
-          apply H4.
-          unfold FlatArray.put, Convertible_word_Nat, HasDefault_word, HasDefault.
-          seprewrite open_constr:(array_index_nat_inbounds (* FIXME: BEDROCK2: Sequencing a failing tactic after a seprewrite backtracks into seprewrite itself; intended? *)
-                                    _ _ _ _ (Z.to_nat (word.unsigned idx)));
-            [ rewrite replace_nth_length; lia | ].
-          instantiate (1 := HasDefault_word).
-          repeat rewrite ?word.ring_morph_mul, ?word.of_Z_unsigned, ?Z2Nat.id by lia.
-          replace (List.firstn (Z.to_nat (word.unsigned idx))
-                               (replace_nth (Z.to_nat (word.unsigned idx)) a val))
-            with (List.firstn (Z.to_nat (word.unsigned idx)) a) by admit.
-          replace (List.skipn (S (Z.to_nat (word.unsigned idx)))
-                              (replace_nth (Z.to_nat (word.unsigned idx)) a val)) with
-              (List.skipn (S (Z.to_nat (word.unsigned idx))) a) by admit.
-          replace (List.hd _ (* FIXME: COQ: replace should allow patterns like change *)
-                           (List.skipn (Z.to_nat (word.unsigned idx))
-                                       (replace_nth (Z.to_nat (word.unsigned idx)) a val))) with
-              val by admit.
-          ecancel_assumption. }
-  Admitted.
+      { eexists; split; cbn.
+        { eexists; split; [ eassumption | reflexivity ]. }
+        { seprewrite_in Hrw H0.
+          once (seprewrite_in
+                  open_constr:(array_index_nat_inbounds
+                                 _ _ (default := default) _ _ (Z.to_nat (word.unsigned (to_word idx)))) H7);
+            [ assumption | ].
+
+          eapply store_word_of_sep.
+          { repeat rewrite ?word.ring_morph_mul, ?word.of_Z_unsigned, ?Z2Nat.id in H6 by lia.
+            ecancel_assumption. }
+          { intros m Hm.
+            apply H4.
+            seprewrite Hrw_put.
+            seprewrite
+              open_constr:(array_index_nat_inbounds
+                             _ _ (default := default) _ _ (Z.to_nat (word.unsigned (to_word idx)))).
+            { rewrite Hput by lia.
+              rewrite List.app_length, List.firstn_length_le by lia.
+              cbn [List.length]; rewrite List.length_skipn.
+              lia. }
+            { rewrite <- Hget0, Hgetput by lia.
+              repeat rewrite ?word.ring_morph_mul, ?word.of_Z_unsigned, ?Z2Nat.id by lia.
+              rewrite Hput by lia.
+
+              rewrite List.firstn_app.
+              rewrite List.firstn_firstn, Min.min_idempotent.
+              rewrite List.firstn_length_le by lia.
+              rewrite Nat.sub_diag; cbn [List.firstn]; rewrite app_nil_r.
+
+              change (val :: ?tl) with (List.app [val] tl).
+              rewrite List.app_assoc, List.skipn_app, List.skipn_all, List.app_nil_l, List.skipn_skipn;
+                rewrite !List.app_length, List.firstn_length_le, (Nat.add_comm _ 1) by lia.
+              - rewrite Nat.sub_diag, Nat.add_0_l.
+                ecancel_assumption.
+              - reflexivity. } } } }
+    Qed.
+  End WordArray.
+
+  Instance Convertible_word_Nat : Convertible word nat :=
+    fun w => Z.to_nat (word.unsigned w).
+  Instance HasDefault_word : HasDefault word :=
+    word.of_Z 0.
+
+  Section WordVectorArray.
+    Definition word_vectorarray_value {n} (addr: address) (a: VectorArray.t word n) : Semantics.mem -> Prop :=
+      array scalar (word.of_Z (Memory.bytes_per_word Semantics.width)) addr (Vector.to_list a).
+
+    Notation repr := word_vectorarray_value.
+    Notation to_list := Vector.to_list.
+    Notation to_word := (proj1_sig (P:=fun idx0 : word => (cast idx0 < _)%nat)).
+    Notation to_nat idx := (Z.to_nat (word.unsigned (to_word idx))).
+
+    Notation get a idx := (VectorArray.get a (proj1_sig idx) (proj2_sig idx)).
+    Notation put a idx v := (VectorArray.put a (proj1_sig idx) (proj2_sig idx) v).
+
+    Lemma WordVectorArray_Hget {n}:
+      forall (a: VectorArray.t word n) idx,
+      exists default,
+        get a idx =
+        List.hd default (List.skipn (to_nat idx) (to_list a)).
+    Proof.
+      intros. exists (word.of_Z 0).
+      apply Vector_nth_hd_skipn.
+      rewrite Fin.to_nat_of_nat; reflexivity.
+    Qed.
+
+    Lemma WordVectorArray_Hput {n} :
+      forall (a : VectorArray.t word n) (idx: {idx : word | (cast idx < n)%nat}) v,
+        to_list (put a idx v) =
+        List.app
+          (List.firstn (to_nat idx) (to_list a))
+          (v :: List.skipn (S (to_nat idx)) (to_list a)).
+    Proof.
+      unfold put.
+      destruct idx as [widx pr]; cbn [proj1_sig proj2_sig].
+      unfold cast, Convertible_word_Nat in *.
+      set (Z.to_nat (word.unsigned widx)) as idx in *.
+      intros.
+      unfold Vector.replace_order; erewrite Vector_to_list_replace by reflexivity.
+      rewrite <- replace_nth_eqn by (rewrite Vector_to_list_length; assumption).
+      rewrite Fin.to_nat_of_nat; reflexivity.
+    Qed.
+
+    Lemma WordVectorArray_Hgetput {n} :
+      forall (a : VectorArray.t word n) (idx: {idx : word | (cast idx < n)%nat}) v,
+        get (put a idx v) idx = v.
+    Proof.
+      unfold get, put, Vector.nth_order, Vector.replace_order.
+      intros; apply Vector_nth_replace.
+    Qed.
+
+    Lemma WordVectorArray_Hrw {n}:
+      forall addr (a: VectorArray.t word n),
+        Lift1Prop.iff1
+          (repr addr a)
+          (array scalar (word.of_Z (Memory.bytes_per_word Semantics.width))
+                 addr (to_list a)).
+    Proof. reflexivity. Qed.
+
+    Lemma compile_word_vectorarray_get {n} :
+      forall (locals: Semantics.locals) (mem: Semantics.mem)
+        tr R functions
+        T (pred: T -> predicate)
+        (a: VectorArray.t word n) (a_ptr: address) a_var idx idx_var k k_impl var pr,
+        (* (pr: (word.unsigned idx < Z.of_nat n)%Z), FIXME if we want this eqn, then indices need to be Z *)
+
+        sep (word_vectorarray_value a_ptr a) R mem ->
+        map.get locals a_var = Some a_ptr ->
+        map.get locals idx_var = Some idx ->
+
+        let v := VectorArray.get a idx pr in
+        (let v := v in
+         <{ Trace := tr;
+            Memory := mem;
+            Locals := map.put locals var v;
+            Functions := functions }>
+         k_impl
+         <{ pred (k v) }>) ->
+        <{ Trace := tr;
+           Memory := mem;
+           Locals := locals;
+           Functions := functions }>
+        cmd.seq
+          (cmd.set
+             var
+             (expr.load
+                access_size.word
+                (expr.op bopname.add
+                         (expr.var a_var)
+                         (expr.op bopname.mul
+                                  (expr.literal (Memory.bytes_per_word Semantics.width))
+                                  (expr.var idx_var)))))
+          k_impl
+        <{ pred (nlet [var] v k) }>.
+    Proof.
+      intros.
+      change v with
+          ((fun a idx => VectorArray.get a (proj1_sig idx) (proj2_sig idx))
+             a (exist (fun idx => cast idx < n)%nat idx pr)).
+      eapply (compile_word_array_get to_list to_word);
+        eauto using WordVectorArray_Hget, WordVectorArray_Hrw.
+      { rewrite Vector_to_list_length.
+        simpl. assumption. }
+    Qed.
+
+    Lemma compile_word_vectorarray_put {n}:
+      forall (locals: Semantics.locals) (mem: Semantics.mem)
+        tr R functions
+        T (pred: T -> predicate)
+        (a: VectorArray.t word n) a_ptr a_var idx idx_var val val_var k k_impl var pr,
+
+        sep (word_vectorarray_value a_ptr a) R mem ->
+        map.get locals a_var = Some a_ptr ->
+        map.get locals idx_var = Some idx ->
+        map.get locals val_var = Some val ->
+
+        let a := (VectorArray.put a idx pr val) in
+        (let a := a in
+         forall mem',
+           sep (word_vectorarray_value a_ptr a) R mem' ->
+           <{ Trace := tr;
+              Memory := mem';
+              Locals := locals;
+              Functions := functions }>
+           k_impl
+           <{ pred (k a) }>) ->
+        <{ Trace := tr;
+           Memory := mem;
+           Locals := locals;
+           Functions := functions }>
+        cmd.seq
+          (cmd.store
+             access_size.word
+             (expr.op bopname.add
+                      (expr.var a_var)
+                      (expr.op bopname.mul
+                               (expr.literal (Memory.bytes_per_word Semantics.width))
+                               (expr.var idx_var)))
+             (expr.var val_var))
+          k_impl
+        <{ pred (nlet [var] a k) }>.
+    Proof.
+      intros.
+      change a0 with
+          ((fun a idx val => VectorArray.put a (proj1_sig idx) (proj2_sig idx) val)
+             a (exist (fun idx => cast idx < n)%nat idx pr) val).
+      eapply (compile_word_array_put
+                to_list to_word
+                (fun a idx => get a idx)
+                (fun a idx v => put a idx v));
+        eauto using WordVectorArray_Hget, WordVectorArray_Hrw,
+        WordVectorArray_Hgetput, WordVectorArray_Hput.
+      rewrite Vector_to_list_length; assumption.
+    Qed.
+  End WordVectorArray.
+
+  Section WordListArray.
+    Definition word_listarray_value (addr: address) (a: ListArray.t word)
+      : Semantics.mem -> Prop :=
+      array scalar (word.of_Z (Memory.bytes_per_word Semantics.width)) addr a.
+
+    Notation repr := word_listarray_value.
+    Notation to_list x := x.
+    Notation to_word x := x.
+    Notation to_nat idx := (Z.to_nat (word.unsigned (to_word idx))).
+
+    Notation get a idx := (ListArray.get a idx).
+    Notation put a idx v := (ListArray.put a idx v).
+
+    Lemma WordListArray_Hget:
+      forall (a: ListArray.t word) idx,
+      exists default,
+        get a idx =
+        List.hd default (List.skipn (to_nat idx) (to_list a)).
+    Proof.
+      intros. exists (word.of_Z 0).
+      unfold get; rewrite <- List.nth_default_eq.
+      apply List.hd_skipn_nth_default.
+    Qed.
+
+    Lemma WordListArray_Hput :
+      forall (a : ListArray.t word) (idx: word) v,
+        (to_nat idx < Datatypes.length a)%nat ->
+        to_list (put a idx v) =
+        List.app
+          (List.firstn (to_nat idx) (to_list a))
+          (v :: List.skipn (S (to_nat idx)) (to_list a)).
+    Proof.
+      unfold put; eauto using replace_nth_eqn.
+    Qed.
+
+    Lemma WordListArray_Hgetput :
+      forall (a : ListArray.t word) (idx: word) v,
+        (to_nat idx < Datatypes.length a)%nat ->
+        get (put a idx v) idx = v.
+    Proof.
+      unfold get, put.
+      intros; apply nth_replace_nth; (assumption || reflexivity).
+    Qed.
+
+    Lemma WordListArray_Hrw:
+      forall addr (a: ListArray.t word),
+        Lift1Prop.iff1
+          (repr addr a)
+          (array scalar (word.of_Z (Memory.bytes_per_word Semantics.width))
+                 addr (to_list a)).
+    Proof. reflexivity. Qed.
+
+    Lemma compile_word_listarray_get :
+      forall (locals: Semantics.locals) (mem: Semantics.mem)
+        tr R functions
+        T (pred: T -> predicate)
+        (a: ListArray.t word) (a_ptr: address) a_var idx idx_var k k_impl var,
+
+        sep (word_listarray_value a_ptr a) R mem ->
+        map.get locals a_var = Some a_ptr ->
+        map.get locals idx_var = Some idx ->
+
+        word.unsigned idx < Z.of_nat (Datatypes.length (id a)) ->
+
+        let v := ListArray.get a idx in
+        (let v := v in
+         <{ Trace := tr;
+            Memory := mem;
+            Locals := map.put locals var v;
+            Functions := functions }>
+         k_impl
+         <{ pred (k v) }>) ->
+        <{ Trace := tr;
+           Memory := mem;
+           Locals := locals;
+           Functions := functions }>
+        cmd.seq
+          (cmd.set
+             var
+             (expr.load
+                access_size.word
+                (expr.op bopname.add
+                         (expr.var a_var)
+                         (expr.op bopname.mul
+                                  (expr.literal (Memory.bytes_per_word Semantics.width))
+                                  (expr.var idx_var)))))
+          k_impl
+        <{ pred (nlet [var] v k) }>.
+    Proof.
+      intros.
+      eapply (compile_word_array_get id id);
+        eauto using WordListArray_Hget, WordListArray_Hrw.
+      pose proof word.unsigned_range idx.
+      unfold id in *; lia.
+    Qed.
+
+    Lemma compile_word_listarray_put :
+      forall (locals: Semantics.locals) (mem: Semantics.mem)
+        tr R functions
+        T (pred: T -> predicate)
+        a a_ptr a_var idx idx_var val val_var k k_impl var,
+
+        sep (word_listarray_value a_ptr a) R mem ->
+        map.get locals a_var = Some a_ptr ->
+        map.get locals idx_var = Some idx ->
+        map.get locals val_var = Some val ->
+
+        (word.unsigned idx < Z.of_nat (List.length a))%Z ->
+
+        let a := (ListArray.put a idx val) in
+        (let a := a in
+         forall mem',
+           sep (word_listarray_value a_ptr a) R mem' ->
+           <{ Trace := tr;
+              Memory := mem';
+              Locals := locals;
+              Functions := functions }>
+           k_impl
+           <{ pred (k a) }>) ->
+        <{ Trace := tr;
+           Memory := mem;
+           Locals := locals;
+           Functions := functions }>
+        cmd.seq
+          (cmd.store
+             access_size.word
+             (expr.op bopname.add
+                      (expr.var a_var)
+                      (expr.op bopname.mul
+                               (expr.literal (Memory.bytes_per_word Semantics.width))
+                               (expr.var idx_var)))
+             (expr.var val_var))
+          k_impl
+        <{ pred (nlet [var] a k) }>.
+    Proof.
+      intros.
+      eapply (compile_word_array_put id id);
+        eauto using WordListArray_Hget, WordListArray_Hput,
+        WordListArray_Hgetput, WordListArray_Hrw.
+      unfold id; pose proof word.unsigned_range idx.
+      lia.
+    Qed.
+  End WordListArray.
+
+  Section WordSizedListArray.
+    Definition word_sizedlistarray_value (addr: address) (len: nat) (a: ListArray.t word)
+      : Semantics.mem -> Prop :=
+      sep (emp (List.length a = len)) (array scalar (word.of_Z (Memory.bytes_per_word Semantics.width)) addr a).
+
+    Notation repr := word_sizedlistarray_value.
+    Notation to_list x := x.
+    Notation to_word x := x.
+    Notation to_nat idx := (Z.to_nat (word.unsigned (to_word idx))).
+
+    Notation get a idx := (ListArray.get a idx).
+    Notation put a idx v := (ListArray.put a idx v).
+
+    Lemma WordSizedListArray_Hrw:
+      forall addr sz (a: ListArray.t word),
+        List.length a = sz ->
+        Lift1Prop.iff1
+          (repr addr sz a)
+          (array scalar (word.of_Z (Memory.bytes_per_word Semantics.width))
+                 addr (to_list a)).
+    Proof. unfold word_sizedlistarray_value.
+       intros. setoid_replace (Datatypes.length a = sz) with True.
+       - apply sep_emp_True_l.
+       - tauto.
+    Qed.
+
+    Lemma WordSizedListArray_length :
+      forall addr sz (a: ListArray.t word) mem R,
+        (repr addr sz a * R)%sep mem -> List.length a = sz.
+    Proof.
+      intros * H; unfold repr in H.
+      eapply proj1. apply sep_emp_l with (m := mem).
+      ecancel_assumption.
+    Qed.
+
+    Lemma compile_word_sizedlistarray_get :
+      forall (locals: Semantics.locals) (mem: Semantics.mem)
+        tr R functions
+        T (pred: T -> predicate)
+        sz (a: ListArray.t word) (a_ptr: address) a_var idx idx_var k k_impl var,
+
+        sep (word_sizedlistarray_value a_ptr sz a) R mem ->
+        map.get locals a_var = Some a_ptr ->
+        map.get locals idx_var = Some idx ->
+
+        word.unsigned idx < Z.of_nat sz ->
+
+        let v := ListArray.get a idx in
+        (let v := v in
+         <{ Trace := tr;
+            Memory := mem;
+            Locals := map.put locals var v;
+            Functions := functions }>
+         k_impl
+         <{ pred (k v) }>) ->
+        <{ Trace := tr;
+           Memory := mem;
+           Locals := locals;
+           Functions := functions }>
+        cmd.seq
+          (cmd.set
+             var
+             (expr.load
+                access_size.word
+                (expr.op bopname.add
+                         (expr.var a_var)
+                         (expr.op bopname.mul
+                                  (expr.literal (Memory.bytes_per_word Semantics.width))
+                                  (expr.var idx_var)))))
+          k_impl
+        <{ pred (nlet [var] v k) }>.
+    Proof.
+      intros.
+      eapply (compile_word_array_get id id _ (fun addr a => repr addr sz a));
+        eauto using WordListArray_Hget.
+      - eapply WordSizedListArray_Hrw, WordSizedListArray_length.
+        eassumption.
+      - unfold id.
+        erewrite WordSizedListArray_length by eassumption.
+        pose proof word.unsigned_range idx.
+        lia.
+    Qed.
+
+    Lemma compile_word_sizedlistarray_put :
+      forall (locals: Semantics.locals) (mem: Semantics.mem)
+        tr R functions
+        T (pred: T -> predicate)
+        sz a a_ptr a_var idx idx_var val val_var k k_impl var,
+
+        sep (word_sizedlistarray_value a_ptr sz a) R mem ->
+        map.get locals a_var = Some a_ptr ->
+        map.get locals idx_var = Some idx ->
+        map.get locals val_var = Some val ->
+
+        (word.unsigned idx < Z.of_nat sz)%Z ->
+
+        let a := (ListArray.put a idx val) in
+        (let a := a in
+         forall mem',
+           sep (word_sizedlistarray_value a_ptr sz a) R mem' ->
+           <{ Trace := tr;
+              Memory := mem';
+              Locals := locals;
+              Functions := functions }>
+           k_impl
+           <{ pred (k a) }>) ->
+        <{ Trace := tr;
+           Memory := mem;
+           Locals := locals;
+           Functions := functions }>
+        cmd.seq
+          (cmd.store
+             access_size.word
+             (expr.op bopname.add
+                      (expr.var a_var)
+                      (expr.op bopname.mul
+                               (expr.literal (Memory.bytes_per_word Semantics.width))
+                               (expr.var idx_var)))
+             (expr.var val_var))
+          k_impl
+        <{ pred (nlet [var] a k) }>.
+    Proof.
+      intros.
+      eapply (compile_word_array_put id id _ _ (fun (addr: word) a => repr addr sz a));
+        eauto using WordListArray_Hget, WordListArray_Hput,
+        WordListArray_Hgetput.
+      - eapply WordSizedListArray_Hrw, WordSizedListArray_length.
+        eassumption.
+      - eapply WordSizedListArray_Hrw.
+        unfold id; rewrite ListArray.put_length.
+        eapply WordSizedListArray_length.
+        eassumption.
+      - unfold id; pose proof word.unsigned_range idx.
+        erewrite WordSizedListArray_length by eassumption.
+        lia.
+    Qed.
+  End WordSizedListArray.
 
   Lemma compile_skip :
     forall (locals: Semantics.locals) (mem: Semantics.mem)
@@ -517,12 +1061,15 @@ Section Compile.
     repeat straightline'. eauto.
   Qed.
 
+  Definition map_remove_many {K V} {M: map.map K V} (ks: list K) m :=
+    List.fold_left map.remove ks m.
+
   Lemma compile_unsets :
     forall vars (locals: Semantics.locals) (mem: Semantics.mem)
       cmd tr functions (pred: predicate),
       (<{ Trace := tr;
           Memory := mem;
-          Locals := List.fold_left map.remove vars locals;
+          Locals := map_remove_many vars locals;
           Functions := functions }>
        cmd
        <{ pred }>) ->
@@ -632,6 +1179,12 @@ Section Compile.
   (*   repeat straightline'. *)
   (* Admitted. *)
 
+  Definition ranged_for_widen_bounds {from idx from' to} :
+    from <= idx < from' ->
+    from' < to ->
+    from <= idx < to.
+  Proof. lia. Qed.
+
   Lemma compile_ranged_for_w {A T}:
     forall tr mem locals functions
       (loop_pred: word -> A -> predicate)
@@ -651,18 +1204,20 @@ Section Compile.
       let v := ranged_for_w from to step body a0 in
       ((* loop body *)
         let lp := lp in
-        forall tr mem locals from',
+        forall tr mem locals from'
+          (Hle: word.unsigned from <= word.unsigned from')
+          (Hlt: word.unsigned from' < word.unsigned to),
           let tok := ExitToken.new true in
-          let a := ranged_for_w from from' step body a0 in
-          (word.unsigned from <= word.unsigned from')%Z ->
-          (word.unsigned from' < word.unsigned to)%Z ->
+          let a := ranged_for_w from from' step
+                               (fun tok idx acc pr =>
+                                  body tok idx acc (ranged_for_widen_bounds pr Hlt)) a0 in
           loop_pred from' a tr mem locals ->
           (<{ Trace := tr;
               Memory := mem;
               Locals := locals;
               Functions := functions }>
            body_impl
-           <{ lp from' (body tok from' a) }>)) ->
+           <{ lp from' (body tok from' a (conj Hle Hlt)) }>)) ->
       (let v := v in
        forall tr mem locals,
          loop_pred to v tr mem locals ->
@@ -691,14 +1246,6 @@ Section Compile.
     cbv zeta.
     repeat straightline'.
   Admitted.
-
-  Instance spec_of_incr : spec_of "incr" :=
-    (forall! (c_ptr : address) (c :cell),
-        (sep (c_ptr ~> c))
-          ===>
-          "incr" @ [c_ptr]
-          ===>
-          (OneCell c_ptr (incr_gallina_spec c))).
 
   Lemma postcondition_func_norets_postcondition_cmd
         {T} spec (x: T) cmd R tr mem locals functions :
@@ -738,15 +1285,16 @@ Section Compile.
   (* Qed. *)
 
   Ltac solve_map_get_goal ::=
-    repeat lazymatch goal with
-           | [ H: map.extends ?m2 ?m1 |- map.get ?m2 ?k = Some ?v ] =>
-             apply (fun p => @map.extends_get _ _ _ m1 m2 k v p H)
-           | [  |- map.get ?m _ = Some ?val ] =>
-             first [ apply map.get_put_same | rewrite map.get_put_diff ]
-           | [  |- map.get ?m _ = None ] =>
-             first [ apply map.get_empty | rewrite map.get_put_diff by congruence ]
-           | [  |- _ <> _ ] => congruence
-           end.
+    progress repeat lazymatch goal with
+                    | [ H: map.extends ?m2 ?m1 |- map.get ?m2 ?k = Some ?v ] =>
+                      apply (fun p => @map.extends_get _ _ _ m1 m2 k v p H)
+                    | [  |- map.get ?m _ = Some ?val ] =>
+                      tryif has_evar val then fail 1 val "has evars" else
+                        first [ apply map.get_put_same | rewrite map.get_put_diff ]
+                    | [  |- map.get ?m _ = None ] =>
+                      first [ apply map.get_empty | rewrite map.get_put_diff by congruence ]
+                    | [  |- _ <> _ ] => congruence
+                    end.
 
   Ltac compile_get_binding :=
     lazymatch goal with
@@ -761,11 +1309,24 @@ Section Compile.
             simple eapply compile_add |
             simple eapply compile_get |
             simple eapply compile_put |
-            simple eapply compile_wordarray_get |
-            simple eapply compile_wordarray_put ].
+            simple eapply compile_word_vectorarray_get |
+            simple eapply compile_word_vectorarray_put |
+            simple eapply compile_word_sizedlistarray_get |
+            simple eapply compile_word_sizedlistarray_put |
+            simple eapply compile_word_listarray_get |
+            simple eapply compile_word_listarray_put ].
+
+   Ltac compile_setup_unfold_spec :=
+     match goal with
+     | [  |- context[?spec] ] =>
+       match type of spec with
+       | spec_of _ => cbv [spec]
+       end
+     end.
 
    Ltac compile_setup :=
      cbv [program_logic_goal_for];
+     compile_setup_unfold_spec;
      (* modified version of a clause in straightline *)
      (intros; WeakestPrecondition.unfold1_call_goal;
       (cbv beta match delta [WeakestPrecondition.call_body]);
@@ -810,7 +1371,7 @@ Section Compile.
      lazymatch type of H with
      | ?x = _ =>
        tryif is_var x then subst x else idtac
-     | match ?x with _ => _ end =>
+     | match ?x with _ => _ end => (* let '(a, b) := … in _ /\ _ *)
        destruct x eqn:?; cleanup_hyp H
      | _ /\ _ =>
        let Hl := fresh "Hl" in
@@ -828,60 +1389,124 @@ UNDEFINED EVARS:
  ?X101685==[semantics semantics_ok len a1 a2 |- Interface.word ?width] (parameter word of
              @word.of_Z) {?word}
  ?X101688==[semantics semantics_ok len a1 a2 (zero:=word.of_Z 0) |-
-             HasDefault word] (parameter v0 of @FlatArray.get) {?v0}
+             HasDefault word] (parameter v0 of @VectorArray.get) {?v0}
  ?X101689==[semantics semantics_ok len a1 a2 (zero:=word.of_Z 0) |-
-             Convertible ?word nat] (parameter k2n of @FlatArray.get) {?k2n}
+             Convertible ?word nat] (parameter k2n of @VectorArray.get) {?k2n}
  ?X101692==[semantics semantics_ok len a1 a2 (zero:=word.of_Z 0) (v:=
-             FlatArray.get a1 zero) |- Convertible ?word nat] (parameter k2n of
-             @FlatArray.put) {?k2n0}
+             VectorArray.get a1 zero) |- Convertible ?word nat] (parameter k2n of
+             @VectorArray.put) {?k2n0}
 TYPECLASSES:?X101685 ?X101688 ?X101689 ?X101692
  *)
 
+   Ltac compile_step :=
+     lazymatch goal with
+     | [  |- let _ := _ in _ ] => intros
+     | [  |- forall _, _ ] => intros
+     | [  |- WeakestPrecondition.cmd _ _ _ _ _ _ ] =>
+       try clear_old_seps;
+       first [compile_custom | compile_basics ]
+     | [  |- sep _ _ _ ] =>
+       autounfold with compiler in *;
+       cbn [fst snd] in *;
+       ecancel_assumption
+     | [  |- map.get _ _ = _ ] =>
+       solve [first [ solve_map_get_goal
+                    | progress subst_lets_in_goal; solve_map_get_goal ] ]
+     | [  |- map.getmany_of_list _ [] = Some _ ] => reflexivity (* FIXME remove? *)
+     | _ => solve [eauto with compiler]
+     end.
+
+   Ltac map_get_bindings m :=
+     let rec loop m acc :=
+         match m with
+         | map.put ?m ?k ?v =>
+           loop m uconstr:((k, v) :: acc)
+         | map.empty => acc
+         end in
+     loop m uconstr:([]).
+
+   Definition map_of_bindings {K V} {M: map.map K V} (bindings: list (K * V)) :=
+     List.fold_left (fun m '(k, v) => map.put m k v) bindings map.empty.
+
+   Lemma map_remove_many_diff {K V} {M: map.map K V} eqb: (* FIXME use maps instead of lists *)
+     forall (b0 b1: list (K * V)) ks,
+       let ks0 := List.map fst b0 in
+       let ks1 := List.map fst b1 in
+       ks = List.filter (fun k0 => negb (List.existsb (eqb k0) ks1)) ks0 ->
+       b1 = List.filter (fun '(k0, b0) => negb (List.existsb (eqb k0) ks)) b0 ->
+       map_remove_many ks (map_of_bindings b0) = map_of_bindings b1.
+   Admitted.
+
+  Ltac solve_map_remove_many :=
+    lazymatch goal with  (* FIXME this needs to handle overwritten bindings *)
+    | [  |- map_remove_many ?ks ?m0 = ?m1 ] =>
+      let b0 := map_get_bindings m0 in
+      let b1 := map_get_bindings m1 in
+      change m0 with (map_of_bindings b0);
+      change m1 with (map_of_bindings b1);
+      apply (map_remove_many_diff String.eqb);
+      [ try (compute; reflexivity) | try reflexivity ]
+    end.
+
    (* FIXME Loop lemma should maybe copy from, to, step into temporaries? *)
-   Definition memcpy (len: word) (a1 a2: FlatArray.t word) :=
+   Program Definition vect_memcpy {n1 n2} (len: word)
+           (a1: VectorArray.t word n1)
+           (a2: VectorArray.t word n2)
+           (pr1: word.unsigned len < Z.of_nat n1)
+           (pr2: word.unsigned len < Z.of_nat n2) :=
      let/n from := word.of_Z 0 in
      let/n step := word.of_Z 1 in
      let/n a2 := ranged_for_w
                   from len step
-                  (fun tok idx a2 =>
-                     let/n v := FlatArray.get a1 idx in
-                     let/n a2 := FlatArray.put a2 idx v in
+                  (fun tok idx a2 Hlt =>
+                     let/n v := VectorArray.get a1 idx _ in
+                     let/n a2 := VectorArray.put a2 idx _ v in
                      (tok, a2)) a2 in
      (a1, a2).
+   Next Obligation.
+     pose proof word.unsigned_range idx.
+     pose proof word.unsigned_range len.
+     unfold cast, Convertible_word_Nat.
+     lia.
+   Qed.
+   Next Obligation.
+     pose proof word.unsigned_range idx.
+     pose proof word.unsigned_range len.
+     unfold cast, Convertible_word_Nat.
+     lia.
+   Qed.
 
-   Definition TwoByteArrays a1_ptr a2_ptr :=
+   Definition TwoVectArrays {n1 n2} a1_ptr a2_ptr :=
      (fun '(a1, a2) (_retvals: list word) =>
-        (word_array_value a1_ptr a1 * word_array_value a2_ptr a2)%sep).
+        (word_vectorarray_value (n := n1) a1_ptr a1 *
+         word_vectorarray_value (n := n2) a2_ptr a2)%sep).
+   Hint Unfold TwoVectArrays : compiler.
 
-   Locate "forall!".
-   Instance spec_of_memcpy : spec_of "memcpy" :=
-     (forall! (len: word) (a1_ptr a2_ptr : address) (a1 a2: FlatArray.t word),
+   Instance spec_of_vect_memcpy : spec_of "vect_memcpy" :=
+     (forall! (len: word) (a1_ptr a2_ptr : address)
+       {n1} (a1: VectorArray.t word n1)
+       {n2} (a2: VectorArray.t word n2)
+       (pr1: word.unsigned len < Z.of_nat n1)
+       (pr2: word.unsigned len < Z.of_nat n2),
          (fun R mem =>
-            (word.unsigned len < Z.of_nat (List.length a1))%Z /\
-            (word.unsigned len < Z.of_nat (List.length a2))%Z /\
-            sep (word_array_value a1_ptr a1 * word_array_value a2_ptr a2)%sep R mem)
+            sep (word_vectorarray_value a1_ptr a1 * word_vectorarray_value a2_ptr a2)%sep R mem)
          ===>
-         "memcpy" @ [len; a1_ptr; a2_ptr]
+         "vect_memcpy" @ [len; a1_ptr; a2_ptr]
          ===>
-         (TwoByteArrays a1_ptr a2_ptr (memcpy len a1 a2))).
+         (TwoVectArrays a1_ptr a2_ptr (vect_memcpy len a1 a2 pr1 pr2))).
 
-   Require Import AdmitAxiom.
-   Derive body SuchThat
-         (let memcpy := ("memcpy", (["len"; "a1"; "a2"], [], body)) in
+   Hint Unfold postcondition_func_norets : compiler.   (* FIXME *)
+   Hint Unfold postcondition_func : compiler.   (* FIXME *)
+
+   Derive vect_memcpy_body SuchThat
+         (let memcpy := ("vect_memcpy", (["len"; "a1"; "a2"], [], vect_memcpy_body)) in
           program_logic_goal_for
             memcpy
             (ltac:(let x := program_logic_goal_for_function
                               memcpy (@nil string) in
                    exact x)))
-         As body_correct.
+         As vect_memcpy_correct.
    Proof.
-     match goal with
-     | [  |- context[?spec] ] =>
-       match type of spec with
-       | spec_of _ => cbv [spec]
-       end
-     end.
-
      compile_setup.
 
      repeat compile_step.
@@ -890,47 +1515,167 @@ TYPECLASSES:?X101685 ?X101688 ?X101689 ?X101692
          tr' = tr /\
          locals' = (∅[["len" ← len]][["a1" ← a1_ptr]][["a2" ← a2_ptr]]
                      [["from" ← idx]][["step" ← v0]]) /\
-         (word_array_value a1_ptr a1 * word_array_value a2_ptr a2 * R)%sep mem')).
+         (word_vectorarray_value a1_ptr a1 * word_vectorarray_value a2_ptr a2 * R)%sep mem')).
 
      { intros * Hpred. cleanup_hyp Hpred.
        repeat apply map.getmany_of_list_cons; compile_step. }
 
      { eauto. }
 
-     { intros * Hle Hlt Hpred. cleanup_hyp Hpred.
-
+     { intros * Hpred; cleanup_hyp Hpred.
        repeat compile_step.
 
-       { lia. }
-       { admit. (* FIXME: There is something smart here: we need to check that the index is in bounds but we modified the array.  Using a vector type instead would keep the information in the type and the statement of Put would specify that the length is preserved.  Alternatively we could do an automatic induction? *)
-       }
+       (* FIXME: without vectors there would be something smart here: we need to check that the index is in bounds but we modified the array.  Using a vector type instead would keep the information in the type and the statement of Put would specify that the length is preserved.  Alternatively we could do an automatic induction? *)
 
-       { apply (compile_unsets ["v"]).
-         apply compile_skip.
+       { eapply compile_unsets; apply compile_skip.
 
-         red; repeat apply conj.
+         repeat red.
+         repeat apply conj.
          + reflexivity.
          + cbn.
-           repeat first [rewrite map.remove_put_diff by congruence |
-                         rewrite map.remove_put_same by congruence |
-                         rewrite map.remove_empty ].
-           reflexivity.
+           solve_map_remove_many.
          + ecancel_assumption. } }
 
      { intros * Hpred. cleanup_hyp Hpred.
        repeat compile_step.
 
        apply compile_skip.
-       do 3 red; repeat apply conj.
+       red.
+       repeat autounfold with compiler.
+
+       repeat apply conj.
        + reflexivity.
        + apply sep_assoc; rewrite sep_emp_l; split.
          * reflexivity.
-         * Hint Unfold TwoByteArrays : compiler.
-           autounfold with compiler.
+         * autounfold with compiler. (* FIXME this autounfold approach doesn't work with temporary predicates generated as part of the derivation *)
            ecancel_assumption. }
    Qed.
 
-   Require Import AdmitAxiom.
+   Definition sizedlist_memcpy (len: word)
+           (a1: ListArray.t word)
+           (a2: ListArray.t word) :=
+     let/n from := word.of_Z 0 in
+     let/n step := word.of_Z 1 in
+     let/n a2 := ranged_for_w
+                  from len step
+                  (fun tok idx a2 Hlt =>
+                     let/n v := ListArray.get a1 idx in
+                     let/n a2 := ListArray.put a2 idx v in
+                     (tok, a2)) a2 in
+     (a1, a2).
+
+   Definition TwoSizedListArrays n1 n2 a1_ptr a2_ptr :=
+     (fun '(a1, a2) (_retvals: list word) =>
+        (word_sizedlistarray_value a1_ptr n1 a1 *
+         word_sizedlistarray_value a2_ptr n2 a2)%sep).
+   Hint Unfold TwoSizedListArrays : compiler.
+
+   Instance spec_of_sizedlist_memcpy : spec_of "sizedlist_memcpy" :=
+     (forall! (len: word) (a1_ptr a2_ptr : address)
+       {n1} (a1: ListArray.t word)
+       {n2} (a2: ListArray.t word)
+       (pr1: word.unsigned len < Z.of_nat n1)
+       (pr2: word.unsigned len < Z.of_nat n2),
+         (fun R mem =>
+            sep (word_sizedlistarray_value a1_ptr n1 a1 *
+                 word_sizedlistarray_value a2_ptr n2 a2)%sep R mem)
+         ===>
+         "sizedlist_memcpy" @ [len; a1_ptr; a2_ptr]
+         ===>
+         (TwoSizedListArrays n1 n2 a1_ptr a2_ptr (sizedlist_memcpy len a1 a2))).
+
+   Derive sizedlist_memcpy_body SuchThat
+         (let memcpy := ("sizedlist_memcpy", (["len"; "a1"; "a2"], [], sizedlist_memcpy_body)) in
+          program_logic_goal_for
+            memcpy
+            (ltac:(let x := program_logic_goal_for_function
+                              memcpy (@nil string) in
+                   exact x)))
+         As sizedlist_memcpy_correct.
+   Proof.
+     compile_setup.
+
+     repeat compile_step.
+
+     eapply compile_ranged_for_w with (loop_pred := (fun idx a2 tr' mem' locals' =>
+         tr' = tr /\
+         locals' = (∅[["len" ← len]][["a1" ← a1_ptr]][["a2" ← a2_ptr]]
+                     [["from" ← idx]][["step" ← v0]]) /\
+         (word_sizedlistarray_value a1_ptr n1 a1 *
+          word_sizedlistarray_value a2_ptr n2 a2 * R)%sep mem')).
+
+     { intros * Hpred. cleanup_hyp Hpred.
+       repeat apply map.getmany_of_list_cons; compile_step. }
+
+     { eauto. }
+
+     { intros * Hle Hlt tok a Hpred; cleanup_hyp Hpred.
+       repeat compile_step.
+
+       { lia. }
+
+       { lia. }
+
+       (* FIXME: without vectors there would be something smart here: we need to check that the index is in bounds but we modified the array.  Using a vector type instead would keep the information in the type and the statement of Put would specify that the length is preserved.  Alternatively we could do an automatic induction? *)
+
+       { eapply compile_unsets; apply compile_skip.
+
+         repeat red.
+         repeat apply conj.
+         + reflexivity.
+         + cbn.
+           solve_map_remove_many.
+         + ecancel_assumption. } }
+
+     { intros * Hpred. cleanup_hyp Hpred.
+       repeat compile_step.
+
+       apply compile_skip.
+       red.
+       repeat autounfold with compiler.
+
+       repeat apply conj.
+       + reflexivity.
+       + apply sep_assoc; rewrite sep_emp_l; split.
+         * reflexivity.
+         * autounfold with compiler. (* FIXME this autounfold approach doesn't work with temporary predicates generated as part of the derivation *)
+           ecancel_assumption. }
+   Qed.
+
+  Program Definition incr_gallina_spec (c: cell) : cell :=
+      let/n one := word.of_Z 1 in
+      let/n from := word.of_Z 3 in
+      let/n to := word.of_Z 5 in
+      let/n step := word.of_Z 1 in
+      let/n tick := word.of_Z 0 in
+      let/n (tick, c) :=
+         ranged_for_w (A := word * cell)
+                      from to step
+                      (fun tok idx acc bounded =>
+                         let '(tick, c) := acc in
+                         let/n v := get c in
+                         let/n v := word.add v idx in
+                         let/n c := put v c in
+                         let/n tick := word.add tick one in
+                         (tok, (tick, c)))
+                      (tick, c) : word * cell in
+      (let/n v := get c in
+       let/n v := word.add v tick in
+       let/n c := put v c in
+       c).
+
+  Print incr_gallina_spec.
+
+  Local Infix "~>" := cell_value.
+
+  Instance spec_of_incr : spec_of "incr" :=
+    (forall! (c_ptr : address) (c :cell),
+        (sep (c_ptr ~> c))
+          ===>
+          "incr" @ [c_ptr]
+          ===>
+          (OneCell c_ptr (incr_gallina_spec c))).
+
    Derive body SuchThat
          (let incr := ("incr", (["c"], [], body)) in
           program_logic_goal_for
@@ -940,14 +1685,13 @@ TYPECLASSES:?X101685 ?X101688 ?X101689 ?X101692
                    exact x)))
          As body_correct.
    Proof.
-     cbv [spec_of_incr].
      compile_setup.
 
      repeat compile_step.
 
      (* FIXME should the variable set always be in the form “extends”?  Or should we add explicit unsets? *)
      eapply compile_ranged_for_w with (loop_pred := (fun idx acc tr' mem' locals' =>
-         let '(P2 tick c) := acc in
+         let '(tick, c) := acc in
          tr' = tr /\
          (* locals' = map.put locals "tick" tick /\ *)
          locals' = (∅[["c" ← c_ptr]][["one" ← v]]
@@ -962,7 +1706,7 @@ TYPECLASSES:?X101685 ?X101688 ?X101689 ?X101692
      { eauto using eq_refl.
        (* + subst locals; rewrite map.put_put_same; reflexivity. *) }
 
-     { intros * Hpred. red in Hpred; cleanup_hyp Hpred.
+     { intros * Hle Hlt tok a0 Hpred. cleanup_hyp Hpred.
 
        repeat compile_step.
 
@@ -976,6 +1720,9 @@ TYPECLASSES:?X101685 ?X101688 ?X101689 ?X101692
        red; repeat apply conj.
        + reflexivity.
        + (* apply extends_eq. *)
+         solve_map_remove_many.
+         cbn.
+
          instantiate (1 := ["v"]).
          cbn.
          (* match goal with *)
